

# Probability Theory Homework 6

Gregory Matsnev

December 23, 2025

## 1 Problem 1

**Problem.** Find the PDF of  $Y = 1 - X^3$ , where  $X$  is the random variable distributed according to the Cauchy law, i. e. with the PDF

$$\phi(x) = \frac{1}{\pi(1+x^2)}$$

**Solution.** Let's express  $x$  in terms of  $y$ :

$$y = 1 - x^3 \iff x^3 = 1 - y \iff x = (1 - y)^{1/3}.$$

Now we'll find the CDF of  $Y$  and then differentiate to get the PDF:

$$F_Y(y) = \mathbb{P}(Y \leq y) = \mathbb{P}(1 - X^3 \leq y) = \mathbb{P}(X^3 \geq 1 - y) = \mathbb{P}(X \geq (1 - y)^{1/3}) = 1 - F_X((1 - y)^{1/3}).$$

$$f_Y(y) = \frac{d}{dy} F_Y(y) = -\frac{d}{dy} F_X((1 - y)^{1/3}) = -f_X((1 - y)^{1/3}) \frac{d}{dy} (1 - y)^{1/3}.$$

$$\frac{d}{dy} (1 - y)^{1/3} = -\frac{1}{3} (1 - y)^{-2/3}, \quad \left| \frac{d}{dy} (1 - y)^{1/3} \right| = \frac{1}{3|1 - y|^{2/3}}.$$

So we get

$$f_Y(y) = f_X((1 - y)^{1/3}) \frac{1}{3|1 - y|^{2/3}}.$$

Now let's substitute the given PDF of  $X$ :

$$f_X((1 - y)^{1/3}) = \frac{1}{\pi(1 + ((1 - y)^{1/3})^2)} = \frac{1}{\pi(1 + |1 - y|^{2/3})}.$$

Finally:

$$f_Y(y) = \frac{1}{\pi(1 + |1 - y|^{2/3})} \cdot \frac{1}{3|1 - y|^{2/3}} = \boxed{\frac{1}{3\pi|1 - y|^{2/3}(1 + |1 - y|^{2/3})}}, \quad y \in \mathbb{R}.$$

## 2 Problem 2

**Problem.** Find the expected value and the variance of the random variable  $Y = 2 - 3 \sin X$ , given that the PDF of  $X$  is

$$\phi(x) = \frac{1}{2} \cos x \text{ for } x \in [-\pi/2, \pi/2]$$

**Solution.**

Let's find  $\mathbb{E}[Y]$ :

$$\begin{aligned}\mathbb{E}[Y] &= \mathbb{E}[2 - 3 \sin X] = \int_{-\pi/2}^{\pi/2} (2 - 3 \sin x) f_X(x) dx = \int_{-\pi/2}^{\pi/2} (2 - 3 \sin x) \frac{1}{2} \cos x dx \\ &= \int_{-\pi/2}^{\pi/2} \cos x dx - \frac{3}{2} \int_{-\pi/2}^{\pi/2} \sin x \cos x dx = \left[ \sin x \right]_{-\pi/2}^{\pi/2} - \frac{3}{2} \left[ \frac{1}{2} \sin^2 x \right]_{-\pi/2}^{\pi/2} = 2.\end{aligned}$$

To find the variance, we need  $\mathbb{E}[Y^2]$ :

$$\begin{aligned}\mathbb{E}[Y^2] &= \mathbb{E}[(2 - 3 \sin X)^2] = \int_{-\pi/2}^{\pi/2} (2 - 3 \sin x)^2 f_X(x) dx = \int_{-\pi/2}^{\pi/2} (4 - 12 \sin x + 9 \sin^2 x) \frac{1}{2} \cos x dx \\ &= 2 \int_{-\pi/2}^{\pi/2} \cos x dx - 6 \int_{-\pi/2}^{\pi/2} \sin x \cos x dx + \frac{9}{2} \int_{-\pi/2}^{\pi/2} \sin^2 x \cos x dx. \\ 2 \int_{-\pi/2}^{\pi/2} \cos x dx &= 2 \left[ \sin x \right]_{-\pi/2}^{\pi/2} = 4, \quad -6 \int_{-\pi/2}^{\pi/2} \sin x \cos x dx = -6 \left[ \frac{1}{2} \sin^2 x \right]_{-\pi/2}^{\pi/2} = 0.\end{aligned}$$

For the last integral, we will use substitution  $u = \sin x$ , so  $du = \cos x dx$ :

$$\frac{9}{2} \int_{-\pi/2}^{\pi/2} \sin^2 x \cos x dx = \frac{9}{2} \int_{-1}^1 u^2 du = \frac{9}{2} \left[ \frac{u^3}{3} \right]_{-1}^1 = 3.$$

So we have

$$\mathbb{E}[Y^2] = 4 + 0 + 3 = 7,$$

and therefore

$\mathbb{E}[Y] = 2, \quad \text{Var}(Y) = \mathbb{E}[Y^2] - (\mathbb{E}[Y])^2 = 7 - 4 = 3.$
---

## 3 Problem 3

**Problem.** The random variable  $X$  is defined on the entire real axis with the probability density  $\phi(x) = \frac{1}{2}e^{-|x|}$ . Find the probability density of the random variable  $Y = X^2$  and its mathematical expectation.

**Solution.**

Since  $Y \geq 0$  and for any  $y > 0$  the equation  $y = x^2$  has two solutions  $x = \pm\sqrt{y}$ , we can use the change-of-variables formula:

$$f_Y(y) = \sum_{x: x^2=y} f_X(x) \left| \frac{dx}{dy} \right| = f_X(\sqrt{y}) \cdot \frac{1}{2\sqrt{y}} + f_X(-\sqrt{y}) \cdot \frac{1}{2\sqrt{y}}, \quad y > 0.$$

Because of the symmetry of  $f_X$ , we have  $f_X(\sqrt{y}) = f_X(-\sqrt{y}) = \frac{1}{2}e^{-\sqrt{y}}$ . Therefore:

$$f_Y(y) = \begin{cases} \frac{e^{-\sqrt{y}}}{\sqrt{y}}, & y > 0, \\ 0, & y \leq 0. \end{cases}$$

The density has an integrable singularity at  $y = 0$ .

For the expectation:

$$\mathbb{E}[Y] = \mathbb{E}[X^2] = \int_{-\infty}^{\infty} x^2 \cdot \frac{1}{2}e^{-|x|} dx = \int_0^{\infty} x^2 e^{-x} dx = \boxed{2}.$$

## 4 Problem 4

**Problem.** Prove formally that if the correlation coefficient  $\rho_{XY}$  of two random variables  $X$  and  $Y$  is equal in absolute value to one, then there is a linear functional relationship between these random variables.

Remember how to prove that  $\text{Cov}(X, Y) \leq \sigma_X \sigma_Y$ .

**Solution.**

Let's assume  $\sigma_X > 0$  and  $\sigma_Y > 0$  (otherwise the correlation isn't defined).

Lets denote the centered variables as  $\tilde{X} = X - \mathbb{E}[X]$  and  $\tilde{Y} = Y - \mathbb{E}[Y]$ .

The correlation coefficient can be written as

$$\rho_{XY} = \frac{\text{Cov}(X, Y)}{\sigma_X \sigma_Y} = \frac{\mathbb{E}[\tilde{X}\tilde{Y}]}{\sqrt{\mathbb{E}[\tilde{X}^2]} \sqrt{\mathbb{E}[\tilde{Y}^2]}}.$$

We know from the Cauchy-Schwarz inequality that

$$|\mathbb{E}[\tilde{X}\tilde{Y}]| \leq \sqrt{\mathbb{E}[\tilde{X}^2]} \sqrt{\mathbb{E}[\tilde{Y}^2]}.$$

Now, if  $|\rho_{XY}| = 1$ , this means we have equality in Cauchy-Schwarz:

$$|\rho_{XY}| = 1 \iff |\mathbb{E}[\tilde{X}\tilde{Y}]| = \sqrt{\mathbb{E}[\tilde{X}^2]} \sqrt{\mathbb{E}[\tilde{Y}^2]}.$$

Lets consider the quadratic form for any  $t \in \mathbb{R}$ :

$$0 \leq \mathbb{E}[(\tilde{Y} - t\tilde{X})^2] = \mathbb{E}[\tilde{Y}^2] - 2t \mathbb{E}[\tilde{X}\tilde{Y}] + t^2 \mathbb{E}[\tilde{X}^2].$$

To find the minimum, let's differentiate with respect to  $t$ :

$$\frac{d}{dt} (\mathbb{E}[\tilde{Y}^2] - 2t \mathbb{E}[\tilde{X}\tilde{Y}] + t^2 \mathbb{E}[\tilde{X}^2]) = -2\mathbb{E}[\tilde{X}\tilde{Y}] + 2t \mathbb{E}[\tilde{X}^2],$$

Setting this to zero gives us

$$t = \frac{\mathbb{E}[\tilde{X}\tilde{Y}]}{\mathbb{E}[\tilde{X}^2]}.$$

Plugging this back in:

$$\mathbb{E}[(\tilde{Y} - t\tilde{X})^2] = \mathbb{E}[\tilde{Y}^2] - \frac{\mathbb{E}[\tilde{X}\tilde{Y}]^2}{\mathbb{E}[\tilde{X}^2]}.$$

But from our condition  $|\rho_{XY}| = 1$ , we have

$$|\mathbb{E}[\tilde{X}\tilde{Y}]| = \sqrt{\mathbb{E}[\tilde{X}^2]}\sqrt{\mathbb{E}[\tilde{Y}^2]} \iff \mathbb{E}[\tilde{X}\tilde{Y}]^2 = \mathbb{E}[\tilde{X}^2]\mathbb{E}[\tilde{Y}^2],$$

which means

$$\mathbb{E}[(\tilde{Y} - t\tilde{X})^2] = \mathbb{E}[\tilde{Y}^2] - \frac{\mathbb{E}[\tilde{X}^2]\mathbb{E}[\tilde{Y}^2]}{\mathbb{E}[\tilde{X}^2]} = 0.$$

Since the expectation of a non-negative random variable is zero, the variable itself must be zero almost surely:

$$\mathbb{E}[(\tilde{Y} - t\tilde{X})^2] = 0 \iff \tilde{Y} - t\tilde{X} = 0 \text{ a.s.} \iff Y - \mathbb{E}[Y] = t(X - \mathbb{E}[X]) \text{ a.s.}$$

So if we set  $c = t$  and  $b = \mathbb{E}[Y] - c\mathbb{E}[X]$ , we get the linear relationship:

$$Y = cX + b \text{ a.s.}$$

## 5 Problem 5

**Problem.** The distribution surface (joint PDF) of the two-dimensional random variable  $(X, Y)$  is a right circular cone, the base of which is a circle centered at the origin with a unit radius. Outside this circle, the joint PDF of this two-dimensional random variable  $(X, Y)$  is zero. Find the joint PDF  $f(x, y)$ , the marginal PDFs and the conditional PDFs  $f_x(y)$  and  $f_y(x)$ . Are the random variables  $X$  and  $Y$  dependent and/or correlated?

**Solution.**

Converting to polar coordinates:

$$1 = \iint_{\mathbb{R}^2} f_{X,Y}(x, y) dx dy = \int_0^{2\pi} \int_0^1 c(1-r) r dr d\theta = 2\pi c \int_0^1 (r-r^2) dr = 2\pi c \left( \frac{1}{2} - \frac{1}{3} \right) = \frac{\pi c}{3},$$

so we have  $c = \frac{3}{\pi}$ . Therefore:

$$f_{X,Y}(x, y) = \frac{3}{\pi} \left( 1 - \sqrt{x^2 + y^2} \right) \mathbf{1}_{\{x^2 + y^2 \leq 1\}}.$$

Now let's find the marginal PDFs. For  $|x| \leq 1$ , we will denote  $a = \sqrt{1 - x^2}$ :

$$f_X(x) = \int_{-\infty}^{\infty} f_{X,Y}(x, y) dy = \int_{-a}^a \frac{3}{\pi} \left( 1 - \sqrt{x^2 + y^2} \right) dy = \frac{6}{\pi} \int_0^a \left( 1 - \sqrt{x^2 + y^2} \right) dy = \frac{6}{\pi} \left( a - \int_0^a \sqrt{x^2 + y^2} dy \right).$$

To evaluate this integral, we will use the antiderivative formula:

$$\int \sqrt{x^2 + y^2} dy = \frac{1}{2} \left( y\sqrt{x^2 + y^2} + x^2 \ln(y + \sqrt{x^2 + y^2}) \right) + C,$$

so we get

$$\int_0^a \sqrt{x^2 + y^2} dy = \frac{1}{2} \left( a\sqrt{x^2 + a^2} + x^2 \ln(a + \sqrt{x^2 + a^2}) - x^2 \ln|x| \right) = \frac{1}{2} \left( a + x^2 \ln(1+a) - x^2 \ln|x| \right),$$

where  $\sqrt{x^2 + a^2} = \sqrt{x^2 + 1 - x^2} = 1$ . Therefore, for  $|x| \leq 1$ :

$$f_X(x) = \frac{6}{\pi} \left( a - \frac{1}{2} \left( a + x^2 \ln(1+a) - x^2 \ln|x| \right) \right) = \frac{3}{\pi} \left( a - x^2 \ln \frac{1+a}{|x|} \right), \quad a = \sqrt{1-x^2},$$

and  $f_X(x) = 0$  for  $|x| > 1$ . At  $x = 0$  we need to take a limit:

$$f_X(0) = \lim_{x \rightarrow 0} \frac{3}{\pi} \left( \sqrt{1-x^2} - x^2 \ln \frac{1+\sqrt{1-x^2}}{|x|} \right) = \frac{3}{\pi}.$$

By symmetry, for  $|y| \leq 1$  with  $b = \sqrt{1-y^2}$ :

$$f_Y(y) = \frac{3}{\pi} \left( b - y^2 \ln \frac{1+b}{|y|} \right), \quad b = \sqrt{1-y^2}, \quad f_Y(y) = 0 \text{ for } |y| > 1.$$

The conditional PDFs are just the ratio of joint to marginal. For  $|x| < 1$ :

$$f_x(y) = f_{Y|X=x}(y) = \frac{f_{X,Y}(x,y)}{f_X(x)} = \frac{\frac{3}{\pi} \left( 1 - \sqrt{x^2 + y^2} \right) \mathbf{1}_{\{x^2 + y^2 \leq 1\}}}{\frac{3}{\pi} \left( \sqrt{1-x^2} - x^2 \ln \frac{1+\sqrt{1-x^2}}{|x|} \right)} = \frac{1 - \sqrt{x^2 + y^2}}{\sqrt{1-x^2} - x^2 \ln \frac{1+\sqrt{1-x^2}}{|x|}} \mathbf{1}_{\{|y| \leq \sqrt{1-x^2}\}}$$

and  $f_x(y) = 0$  otherwise. Similarly, for  $|y| < 1$ :

$$f_y(x) = f_{X|Y=y}(x) = \frac{f_{X,Y}(x,y)}{f_Y(y)} = \frac{1 - \sqrt{x^2 + y^2}}{\sqrt{1-y^2} - y^2 \ln \frac{1+\sqrt{1-y^2}}{|y|}} \mathbf{1}_{\{|x| \leq \sqrt{1-y^2}\}},$$

and  $f_y(x) = 0$  otherwise.

Now let's check if  $X$  and  $Y$  are independent. At the origin:

$$f_{X,Y}(0,0) = \frac{3}{\pi}, \quad f_X(0) = \frac{3}{\pi}, \quad f_Y(0) = \frac{3}{\pi}, \quad f_X(0)f_Y(0) = \frac{9}{\pi^2} \neq \frac{3}{\pi},$$

so  $X$  and  $Y$  are dependent.

What about correlation? By symmetry:

$$\mathbb{E}[X] = \iint_{\mathbb{R}^2} x f_{X,Y}(x,y) dx dy = \iint_{\mathbb{R}^2} (-x) f_{X,Y}(-x,y) dx dy = -\mathbb{E}[X] \implies \mathbb{E}[X] = 0,$$

$$\mathbb{E}[Y] = \iint_{\mathbb{R}^2} y f_{X,Y}(x,y) dx dy = \iint_{\mathbb{R}^2} (-y) f_{X,Y}(x,-y) dx dy = -\mathbb{E}[Y] \implies \mathbb{E}[Y] = 0,$$

$$\mathbb{E}[XY] = \iint_{\mathbb{R}^2} xy f_{X,Y}(x, y) dx dy = \iint_{\mathbb{R}^2} (-x) y f_{X,Y}(-x, y) dx dy = -\mathbb{E}[XY] \implies \mathbb{E}[XY] = 0,$$

So we have

$$\text{Cov}(X, Y) = \mathbb{E}[XY] - \mathbb{E}[X]\mathbb{E}[Y] = 0, \quad \rho_{XY} = 0.$$

So to summarize:

$$\begin{aligned} f_{X,Y}(x, y) &= \frac{3}{\pi} \left(1 - \sqrt{x^2 + y^2}\right) \mathbf{1}_{\{x^2 + y^2 \leq 1\}}, \\ f_X(x) &= \frac{3}{\pi} \left( \sqrt{1 - x^2} - x^2 \ln \frac{1 + \sqrt{1 - x^2}}{|x|} \right) \mathbf{1}_{\{|x| \leq 1\}}, \\ f_Y(y) &= \frac{3}{\pi} \left( \sqrt{1 - y^2} - y^2 \ln \frac{1 + \sqrt{1 - y^2}}{|y|} \right) \mathbf{1}_{\{|y| \leq 1\}}, \\ f_x(y) &= \frac{1 - \sqrt{x^2 + y^2}}{\sqrt{1 - x^2} - x^2 \ln \frac{1 + \sqrt{1 - x^2}}{|x|}} \mathbf{1}_{\{|x| < 1, |y| \leq \sqrt{1 - x^2}\}}, \\ f_y(x) &= \frac{1 - \sqrt{x^2 + y^2}}{\sqrt{1 - y^2} - y^2 \ln \frac{1 + \sqrt{1 - y^2}}{|y|}} \mathbf{1}_{\{|y| < 1, |x| \leq \sqrt{1 - y^2}\}}, \\ X, Y \text{ dependent}, \quad \text{Cov}(X, Y) &= 0, \quad \rho_{XY} = 0. \end{aligned}$$

## 6 Problem 6

**Problem.** Let  $X$  and  $Y$  be continuous random variables with a (spherically symmetric) joint PDF of the form  $f(x, y) = g(x^2 + y^2)$  for some function  $g$ . Let  $(R, \theta)$  be the polar coordinates of  $(X, Y)$ , so that  $R^2 = X^2 + Y^2$  is the squared distance from the origin and  $\theta$  is the angle  $\in [0, 2\pi)$ , with  $X = R \cos \theta$ ,  $Y = R \sin \theta$ .

a) Prove that  $R$  and  $\theta$  are independent and explain intuitively why this result makes sense;

b) What is the joint PDF of  $(R, \theta)$  if  $(X, Y)$  is Uniform on the unit disk, i. e.  $x^2 + y^2 \leq 1$ ? If  $X, Y$  are i. i. d.  $N(0, 1)$ ?

**Solution.**

**Part (a):** Let's convert to polar coordinates:  $x = r \cos \theta$ ,  $y = r \sin \theta$  where  $r \geq 0$  and  $\theta \in [0, 2\pi)$ .

The Jacobian of the transformation is

$$\left| \frac{\partial(x, y)}{\partial(r, \theta)} \right| = \begin{vmatrix} \cos \theta & -r \sin \theta \\ \sin \theta & r \cos \theta \end{vmatrix} = r, \quad dx dy = r dr d\theta.$$

Using the change of variables formula:

$$f_{R,\Theta}(r, \theta) = f_{X,Y}(r \cos \theta, r \sin \theta) \left| \frac{\partial(x, y)}{\partial(r, \theta)} \right| = g((r \cos \theta)^2 + (r \sin \theta)^2) r = g(r^2) r, \quad r \geq 0, \theta \in [0, 2\pi).$$

Notice that the joint PDF doesn't depend on  $\theta$  at all. Let's verify this leads to independence. The normalization gives:

$$1 = \int_0^{2\pi} \int_0^\infty f_{R,\Theta}(r, \theta) dr d\theta = \int_0^{2\pi} \int_0^\infty g(r^2) r dr d\theta = 2\pi \int_0^\infty g(r^2) r dr,$$

so

$$\int_0^\infty g(r^2) r dr = \frac{1}{2\pi}.$$

The marginal of  $\Theta$  is:

$$f_\Theta(\theta) = \int_0^\infty f_{R,\Theta}(r, \theta) dr = \int_0^\infty g(r^2) r dr = \frac{1}{2\pi}, \quad \theta \in [0, 2\pi).$$

The marginal of  $R$  is:

$$f_R(r) = \int_0^{2\pi} f_{R,\Theta}(r, \theta) d\theta = \int_0^{2\pi} g(r^2) r d\theta = 2\pi r g(r^2), \quad r \geq 0.$$

We can check:

$$f_R(r)f_\Theta(\theta) = (2\pi r g(r^2)) \left( \frac{1}{2\pi} \right) = g(r^2) r = f_{R,\Theta}(r, \theta),$$

so  $R$  and  $\Theta$  are independent. Since the distribution is spherically symmetric, it is rotationally invariant, which means the angle is uniformly distributed and independent of the distance from the origin.

**Part (b):** Let's apply this to the two specific cases.

**Uniform on the unit disk:** Here  $f_{X,Y}(x, y) = \frac{1}{\pi} \mathbf{1}_{\{x^2 + y^2 \leq 1\}}$ , which has the form  $g(x^2 + y^2)$  with  $g(u) = \frac{1}{\pi} \mathbf{1}_{\{u \leq 1\}}$ . So:

$$f_{R,\Theta}(r, \theta) = \frac{r}{\pi} \mathbf{1}_{\{0 \leq r \leq 1\}} \mathbf{1}_{\{0 \leq \theta < 2\pi\}}.$$

The marginals are:

$$f_\Theta(\theta) = \int_0^1 \frac{r}{\pi} dr = \frac{1}{2\pi}, \quad 0 \leq \theta < 2\pi,$$

$$f_R(r) = \int_0^{2\pi} \frac{r}{\pi} d\theta = 2r, \quad 0 \leq r \leq 1.$$

**i.i.d.  $N(0, 1)$ :** When  $X, Y$  are independent standard normals, we have

$$f_{X,Y}(x, y) = \frac{1}{2\pi} \exp\left(-\frac{x^2 + y^2}{2}\right) = \frac{1}{2\pi} \exp\left(-\frac{r^2}{2}\right),$$

so  $g(u) = \frac{1}{2\pi} e^{-u/2}$ . This gives:

$$f_{R,\Theta}(r, \theta) = \frac{r}{2\pi} \exp\left(-\frac{r^2}{2}\right) \mathbf{1}_{\{r \geq 0\}} \mathbf{1}_{\{0 \leq \theta < 2\pi\}}.$$

The marginals are:

$$f_{\Theta}(\theta) = \int_0^{\infty} \frac{r}{2\pi} e^{-r^2/2} dr = \frac{1}{2\pi}, \quad 0 \leq \theta < 2\pi,$$

$$f_R(r) = \int_0^{2\pi} \frac{r}{2\pi} e^{-r^2/2} d\theta = r e^{-r^2/2}, \quad r \geq 0.$$

$$\begin{aligned} f_{R,\Theta}(r, \theta) &= g(r^2) r, \quad r \geq 0, \ 0 \leq \theta < 2\pi, \\ f_{R,\Theta}(r, \theta) &= \frac{r}{\pi} \mathbf{1}_{\{0 \leq r \leq 1\}} \mathbf{1}_{\{0 \leq \theta < 2\pi\}}, \\ f_{R,\Theta}(r, \theta) &= \frac{r}{2\pi} \exp\left(-\frac{r^2}{2}\right) \mathbf{1}_{\{r \geq 0\}} \mathbf{1}_{\{0 \leq \theta < 2\pi\}}. \end{aligned}$$